added wasm stuff to compiler file until we get formalization

src/compiler.v
@@ -1,11 +1,23 @@
 Require Import wacket.
 Require Import observable.
+Require Import String. Local Open Scope string.
+
+(* this should be taken from an open source project*)
+Inductive wasm : Type :=
+
+.
+
+Reserved Notation " t 'c==>' n " (at level 50, left associativity).
+Inductive wasmEval: wasm -> observable -> Prop :=
+    
+where " t 'c==>' n " := (wasmEval t n).
+
+
 
 Inductive compilerResult : Type :=
 | Succ : wasm -> compilerResult
 | Error : string -> compilerResult
 .
 
-
 (* the compiler from wacket to wasm, if *)
-Fixpoint wasmCompiler (source : wack) : compilerResult := Error "not implemented" .
+Fixpoint wasmCompiler (source : dupe) := Error "not implemented" .
